TestVectorsAwsCryptographicMaterialProviders/runtimes/java/src/main/smithy-generated/software/amazon/cryptography/materialProvidersTestVectorKeys/model/KmsRsaKeyring.java
@@ -4,16 +4,24 @@
 package software.amazon.cryptography.materialProvidersTestVectorKeys.model;
 
 import java.util.Objects;
+import software.amazon.awssdk.services.kms.model.EncryptionAlgorithmSpec;
 
 public class KmsRsaKeyring {
   private final String keyId;
 
+  private final EncryptionAlgorithmSpec encryptionAlgorithm;
+
   protected KmsRsaKeyring(BuilderImpl builder) {
     this.keyId = builder.keyId();
+    this.encryptionAlgorithm = builder.encryptionAlgorithm();
   }
 
   public String keyId() {
     return this.keyId;
+  }
+
+  public EncryptionAlgorithmSpec encryptionAlgorithm() {
+    return this.encryptionAlgorithm;
   }
 
   public Builder toBuilder() {
@@ -29,17 +37,24 @@ public class KmsRsaKeyring {
 
     String keyId();
 
+    Builder encryptionAlgorithm(EncryptionAlgorithmSpec encryptionAlgorithm);
+
+    EncryptionAlgorithmSpec encryptionAlgorithm();
+
     KmsRsaKeyring build();
   }
 
   static class BuilderImpl implements Builder {
     protected String keyId;
 
+    protected EncryptionAlgorithmSpec encryptionAlgorithm;
+
     protected BuilderImpl() {
     }
 
     protected BuilderImpl(KmsRsaKeyring model) {
       this.keyId = model.keyId();
+      this.encryptionAlgorithm = model.encryptionAlgorithm();
     }
 
     public Builder keyId(String keyId) {
@@ -51,9 +66,21 @@ public class KmsRsaKeyring {
       return this.keyId;
     }
 
+    public Builder encryptionAlgorithm(EncryptionAlgorithmSpec encryptionAlgorithm) {
+      this.encryptionAlgorithm = encryptionAlgorithm;
+      return this;
+    }
+
+    public EncryptionAlgorithmSpec encryptionAlgorithm() {
+      return this.encryptionAlgorithm;
+    }
+
     public KmsRsaKeyring build() {
       if (Objects.isNull(this.keyId()))  {
         throw new IllegalArgumentException("Missing value for required field `keyId`");
+      }
+      if (Objects.isNull(this.encryptionAlgorithm()))  {
+        throw new IllegalArgumentException("Missing value for required field `encryptionAlgorithm`");
       }
       return new KmsRsaKeyring(this);
     }
