TestVectorsAwsCryptographicMaterialProviders/runtimes/net/Generated/KeyVectors/KmsRsaKeyring.cs
@@ -5,6 +5,7 @@ using System;
  using AWS.Cryptography.MaterialProvidersTestVectorKeys; namespace AWS.Cryptography.MaterialProvidersTestVectorKeys {
  public class KmsRsaKeyring {
  private string _keyId ;
+ private Amazon.KeyManagementService.EncryptionAlgorithmSpec _encryptionAlgorithm ;
  public string KeyId {
  get { return this._keyId; }
  set { this._keyId = value; }
@@ -12,8 +13,16 @@ using System;
  public bool IsSetKeyId () {
  return this._keyId != null;
 }
+ public Amazon.KeyManagementService.EncryptionAlgorithmSpec EncryptionAlgorithm {
+ get { return this._encryptionAlgorithm; }
+ set { this._encryptionAlgorithm = value; }
+}
+ public bool IsSetEncryptionAlgorithm () {
+ return this._encryptionAlgorithm != null;
+}
  public void Validate() {
  if (!IsSetKeyId()) throw new System.ArgumentException("Missing value for required property 'KeyId'");
+ if (!IsSetEncryptionAlgorithm()) throw new System.ArgumentException("Missing value for required property 'EncryptionAlgorithm'");
 
 }
 }
